feat: setup LTL

example/MultiWorkerWithQueue.thy
@@ -44,12 +44,94 @@ fun step :: "'val StepFunction" where
 | "step _ st _ = (st, {})"
 
 inductive execute :: "'val StepFunction \<Rightarrow> 'val State \<Rightarrow> (Node \<times> (Node, 'val Message) Event) list \<Rightarrow> (Node \<times> 'val Message) set \<Rightarrow> bool" where
-  exec_empty: "execute step st [] {}"
-| exec_step: "\<lbrakk> execute step st events msgs;
+  exec_empty: "execute step' st [] {}"
+| exec_step: "\<lbrakk> execute step' st events msgs;
     valid_event event proc msgs;
-    step proc st event = (st', ns);
+    step' proc st event = (st', ns);
     events' = events @ [(proc, event)];
     msgs' = msgs \<union> (\<lambda>msg. (proc, msg)) ` ns
-  \<rbrakk> \<Longrightarrow> execute step st' events' msgs'"
+  \<rbrakk> \<Longrightarrow> execute step' st' events' msgs'"
+
+inductive execute_step where
+  exec_step: "\<lbrakk> valid_event event proc msgs;
+    step' proc st event = (st', ns);
+    events' = events @ [(proc, event)];
+    msgs' = msgs \<union> (\<lambda>msg. (proc,msg)) ` ns
+  \<rbrakk> \<Longrightarrow> execute_step step' (st,events,msgs) (st',events',msgs')"
+
+definition execute_steps where
+  "execute_steps step' \<equiv> rtranclp (execute_step step')"
+
+type_synonym 'val world = "'val State \<times> (Node \<times> (Node, 'val Message) Event) list \<times> (Node \<times> 'val Message) set"
+
+type_synonym 'val Predicate = "'val world \<Rightarrow> bool"
+datatype 'val Prop
+  = Atom "'val Predicate"
+  | Not "'val Prop"
+  | Or "'val Prop" "'val Prop"  (infix "[\<or>]" 40)
+  | Next "'val Prop"  ("\<circle> _" [100] 80)
+  | Until "'val Prop" "'val Prop"  (infix "[U]" 40)
+
+definition And (infix "[\<and>]" 45) where
+  "And p q = Not (Not p [\<or>] Not q)"
+
+definition true where
+  "true \<equiv> Atom (\<lambda>_. True)"
+
+definition false where
+  "false \<equiv> Atom (\<lambda>_. False)"
+
+definition Release :: "'val Prop \<Rightarrow> 'val Prop \<Rightarrow> 'val Prop" (infix "[R]" 50) where
+  "\<phi> [R] \<psi> \<equiv> Not (Not \<phi> [U] Not \<psi>)"
+
+definition Finally :: "'val Prop \<Rightarrow> 'val Prop" ("\<diamondsuit> _" [100] 80) where
+  "\<diamondsuit>\<phi> \<equiv> true [U] \<phi>"
+
+definition Globally :: "'val Prop \<Rightarrow> 'val Prop" ("\<box> _" [100] 80) where
+  "\<box>\<phi> \<equiv> false [R] \<phi>"
+
+definition Paths :: "'val world \<Rightarrow> (nat \<Rightarrow> 'val world) set" where
+  "Paths w = {\<pi>. \<pi> 0 = w \<and> (\<forall>i. execute_step step (\<pi> i) (\<pi> (i+1)))}"
+
+definition suffix where
+  "suffix k \<pi> \<equiv> \<lambda>i. \<pi> (k+i)"
+
+primrec semantical_path :: "(nat \<Rightarrow> 'val world) \<Rightarrow> 'val Prop \<Rightarrow> bool" (infix "\<Turnstile>p" 60) where
+  "(\<pi> \<Turnstile>p Atom p) = p (\<pi> 0)"
+| "(\<pi> \<Turnstile>p Not p) = (\<not> (\<pi> \<Turnstile>p p))"
+| "(\<pi> \<Turnstile>p Or p q) = (\<pi> \<Turnstile>p p \<or> \<pi> \<Turnstile>p q)"
+| "(\<pi> \<Turnstile>p Next p) = (suffix 1 \<pi> \<Turnstile>p p)"
+| "(\<pi> \<Turnstile>p Until p q) = (\<exists>i. suffix i \<pi> \<Turnstile>p q \<and> (\<forall>j. i < j \<longrightarrow> suffix j \<pi> \<Turnstile>p p))"
+
+definition semantical :: "'val world \<Rightarrow> 'val Prop \<Rightarrow> bool" (infix "\<Turnstile>" 60) where
+  "w \<Turnstile> p = (\<forall>\<pi>. \<pi> 0 = w \<and> \<pi> \<Turnstile>p p)"
+
+lemma not_true_iff_false [simp]:
+  "w \<Turnstile> Not true = w \<Turnstile> false"
+  by (simp add: semantical_def true_def false_def)
+
+lemma next_not_compat [simp]:
+  "w \<Turnstile> \<circle> (Not \<phi>) = w \<Turnstile> Not (\<circle> \<phi>)"
+  by (simp add: semantical_def)
+
+lemma path_until_release_iff:
+  "\<pi> \<Turnstile>p (p [R] q) = (\<not> \<pi> \<Turnstile>p (Not p [U] Not q))"
+  "\<pi> \<Turnstile>p (p [U] q) = (\<not> \<pi> \<Turnstile>p (Not p [R] Not q))"
+  apply (simp add: Release_def)
+  apply (simp add: Release_def)
+  done
+
+lemma Globally_and_Finally:
+  "\<pi> \<Turnstile>p \<box>\<phi> = \<pi> \<Turnstile>p Not (\<diamondsuit> (Not \<phi>))"
+  unfolding Globally_def Finally_def
+proof-
+  have "\<pi> \<Turnstile>p Not (true [U] Not \<phi>) = (\<not> \<pi> \<Turnstile>p (true [U] Not \<phi>))"
+    by simp
+  also have "\<dots> = (\<pi> \<Turnstile>p (Not true [R] Not (Not \<phi>)))"
+    using path_until_release_iff(2) by blast
+  also have "\<dots> = (\<pi> \<Turnstile>p (false [R] \<phi>))"
+    by (simp add: false_def path_until_release_iff(1) true_def)
+  finally show "\<pi> \<Turnstile>p (false [R] \<phi>) = \<pi> \<Turnstile>p Prop.Not (true [U] Prop.Not \<phi>)" by simp
+qed
 
 end
